\noindent Étudier la convergence des séries $\sum u_n$ de terme général suivant :

\begin{enumerate}
    \item $\displaystyle u_n = \frac{1}{\sqrt{n}} ln(1 + \frac{1}{\sqrt{n}})$.
    \item $\displaystyle u_n = (1 + \frac{1}{n})^n - e$.
    \item $\displaystyle u_n = (\frac{n}{n + 1})^{n^2}$.
    \item $\displaystyle u_n = \frac{(n!)^2}{(2n)!} a^n$ avec $a \in \ensR_+^*$.
    \item $\displaystyle u_n = \frac{(-1)^n ln(n)}{n}$.
    \item $\displaystyle u_n = \frac{n^42^{-n^2} + (-1)^n}{\sqrt{n}}$.
    \item $\displaystyle u_n = ln(1 + \frac{(-1)^n}{2n + 1})$.
\end{enumerate}